WIP: Progress on incr example

fairness/examples/yesno_incr/yesno_incr_adequacy.v
@@ -1,3 +1,4 @@
+From Paco Require Import paco1 paco2 pacotac.
 From iris.base_logic.lib Require Import invariants.
 From iris.algebra Require Import excl_auth.
 From iris.proofmode Require Import tactics.
@@ -8,8 +9,252 @@ From trillium.fairness.heap_lang Require Export lang lifting tactics.
 From trillium.fairness.heap_lang Require Import notation.
 From trillium.fairness Require Import trace_utils.
 From trillium.fairness.examples.yesno_incr Require Import yesno_incr3.
-
 From stdpp Require Import finite.
+
+(* TODO: Move prerequisites *)
+Lemma infinite_trace_after'' {S T} n (tr tr' : trace S T) :
+  after n tr = Some tr' → infinite_trace tr → infinite_trace tr'.
+Proof.
+  intros Hafter Hinf m. specialize (Hinf (n+m)).
+  rewrite after_sum' in Hinf. rewrite Hafter in Hinf. done.
+Qed.
+
+Lemma trace_eventually_cons {S T} s l (tr : trace S T) P :
+  trace_eventually tr P → trace_eventually (s -[l]-> tr) P.
+Proof. intros [n HP]. by exists (Datatypes.S n). Qed.
+
+(* Definition yesno_aux_progress n b (auxtr : auxtrace the_model) := *)
+(*   trace_eventually auxtr (ls_under ∘ (λ s _, s = (n,b))). *)
+Lemma trace_eventually_stutter_preserves `(LM : LiveModel Λ FM)
+      (mtr : mtrace FM)
+      (auxtr : auxtrace LM) P :
+  upto_stutter ls_under Ul auxtr mtr →
+  trace_eventually mtr P →
+  trace_eventually auxtr (λ s l, P (ls_under s) (l ≫= Ul)).
+Proof.
+  intros Hstutter [n Heventually].
+  revert mtr auxtr Hstutter Heventually.
+  induction n as [|n IHn]; intros mtr auxtr Hstutter Heventually.
+  - punfold Hstutter; [|apply upto_stutter_mono].
+    induction Hstutter.
+    + rewrite /pred_at in Heventually. simpl in *. exists 0. rewrite /pred_at. simpl in *. done.
+    + destruct (IHHstutter Heventually) as [n Heventually'].
+      exists (1 + n). rewrite /pred_at. rewrite after_sum'. simpl.
+      done.
+    + rewrite /pred_at in Heventually. simpl in *. exists 0. rewrite /pred_at. simpl.
+      simplify_eq. rewrite H0. done.
+  - punfold Hstutter; [|apply upto_stutter_mono].
+    induction Hstutter.
+    + rewrite /pred_at in Heventually. simpl in *. exists 0. rewrite /pred_at. simpl in *. done.
+    + destruct (IHHstutter Heventually) as [n' Heventually'].
+      exists (1 + n'). rewrite /pred_at. rewrite after_sum'. simpl.
+      done.
+    + apply trace_eventually_cons.
+      assert (pred_at str n P) as Heventually'.
+      { rewrite /pred_at in Heventually.
+        simpl in *. done. }
+      eapply IHn; [|done].
+      rewrite /upaco2 in H1. destruct H1; [done|done].
+Qed.
+
+Lemma even_odd_False n : Nat.even n → Nat.odd n → False.
+Proof.
+  intros Heven Hodd. rewrite -Nat.negb_odd in Heven.
+  apply Is_true_true_1 in Heven.
+  apply Is_true_true_1 in Hodd.
+  rewrite Hodd in Heven.
+  done.
+Qed.
+
+Lemma even_not_odd n : Nat.even n → ¬ Nat.odd n.
+Proof. intros Heven Hodd. by eapply even_odd_False. Qed.
+
+Lemma odd_not_even n : Nat.odd n → ¬ Nat.even n.
+Proof. intros Heven Hodd. by eapply even_odd_False. Qed.
+
+(* TODO: move to fairness.v *)
+Lemma mtrace_valid_after `{M : FairModel} (mtr mtr' : mtrace M) k :
+  after k mtr = Some mtr' → mtrace_valid mtr → mtrace_valid mtr'.
+Proof.
+  revert mtr mtr'.
+  induction k; intros mtr mtr' Hafter Hvalid.
+  { destruct mtr'; simpl in *; by simplify_eq. }
+  punfold Hvalid.
+  inversion Hvalid as [|??? Htrans Hval']; simplify_eq.
+  eapply IHk; [done|].
+  by inversion Hval'.
+Qed.
+
+Lemma rel_finitary_sim_rel_with_user_sim_rel `{LM:LiveModel Λ Mdl}
+      `{EqDecision (mstate LM)} `{EqDecision (mlabel LM)}
+      `{Countable (locale Λ)} ξ :
+  rel_finitary (sim_rel LM) → rel_finitary (sim_rel_with_user LM ξ).
+Proof.
+  intros Hrel. eapply rel_finitary_impl; [|done]. by intros ex aux [Hsim _].
+Qed.
+
+
+Definition rel_always_holds {Σ} `{LM:LiveModel heap_lang M} `{!heapGS Σ LM}
+           (s:stuckness) (ξ : execution_trace heap_lang → finite_trace M
+                  (option $ fmrole M) → Prop) (c1:cfg heap_lang)
+           (c2:live_model_to_model LM) : iProp Σ :=
+  ∀ ex atr c,
+    ⌜valid_system_trace ex atr⌝ -∗
+    ⌜trace_starts_in ex c1⌝ -∗
+    ⌜trace_starts_in atr c2⌝ -∗
+    ⌜trace_ends_in ex c⌝ -∗
+    ⌜∀ ex' atr' oζ ℓ, trace_contract ex oζ ex' →
+                      trace_contract atr ℓ atr' →
+                      ξ ex' (map_underlying_trace atr')⌝ -∗
+    ⌜∀ e2, s = NotStuck → e2 ∈ c.1 → not_stuck e2 c.2⌝ -∗
+    state_interp ex atr -∗
+    posts_of c.1 ((λ _, 0%nat ↦M ∅) :: ((λ '(tnew, e), fork_post (locale_of tnew e)) <$> (prefixes_from c1.1 (drop (length c1.1) c.1)))) -∗
+    |={⊤, ∅}=> ⌜ξ ex (map_underlying_trace atr)⌝.
+
+Theorem strong_simulation_adequacy Σ `(LM:LiveModel heap_lang M)
+    `{!heapGpreS Σ LM} (s: stuckness) (e1 : expr) σ1 (s1: M) (FR: gset _)
+    (ξ : execution_trace heap_lang → finite_trace M (option $ fmrole M) →
+         Prop) :
+  rel_finitary (sim_rel_with_user LM ξ) →
+  live_roles M s1 ≠ ∅ ->
+  (∀ `{Hinv : !heapGS Σ LM},
+    ⊢ |={⊤}=>
+       (* state_interp (trace_singleton ([e1], σ1)) (trace_singleton (initial_ls (LM := LM) s1 0%nat)) ∗ *)
+       ([∗ map] l ↦ v ∈ heap σ1, mapsto l (DfracOwn 1) v) -∗
+       frag_model_is s1 -∗
+       frag_free_roles_are (FR ∖ live_roles _ s1) -∗
+       has_fuels (Σ := Σ) 0%nat (gset_to_gmap (LM.(lm_fl) s1) (M.(live_roles) s1)) ={⊤}=∗
+       WP e1 @ s; locale_of [] e1; ⊤ {{ v, 0%nat ↦M ∅ }} ∗
+       rel_always_holds s ξ ([e1], σ1) (initial_ls (LM := LM) s1 0%nat)) ->
+  continued_simulation (sim_rel_with_user LM ξ) (trace_singleton ([e1], σ1)) (trace_singleton (initial_ls (LM := LM) s1 0%nat)).
+Proof.
+  intros Hfin Hfevol H.
+  apply (wp_strong_adequacy heap_lang LM Σ s); first by eauto.
+  iIntros (?) "".
+  iMod (gen_heap_init (heap σ1)) as (genheap)" [Hgen [Hσ _]]".
+  iMod (model_state_init s1) as (γmod) "[Hmoda Hmodf]".
+  iMod (model_mapping_init s1) as (γmap) "[Hmapa Hmapf]".
+  iMod (model_fuel_init s1) as (γfuel) "[Hfuela Hfuelf]".
+  iMod (model_free_roles_init s1 (FR ∖ live_roles _ s1)) as (γfr) "[HFR Hfr]".
+  set (distG :=
+         {|
+          heap_fairnessGS := {|
+                              fairness_model_name := γmod;
+                              fairness_model_mapping_name := γmap;
+                              fairness_model_fuel_name := γfuel;
+                              fairness_model_free_roles_name := γfr;
+                              |}
+         |}).
+  iMod (H distG) as "Hwp". clear H.
+  iExists state_interp, (λ _, 0%nat ↦M ∅)%I, fork_post.
+  iSplitR.
+  { unfold config_wp. iIntros "!>!>" (???????) "?". done. }
+  (* iAssert (state_interp with "[Hgen Hmoda Hmodf Hmapa Hfuela HFR] Hfr [Hfuelf Hmapf]"). *)
+  (* { iFrame "Hmodf". unfold state_interp. simpl. iFrame. iExists {[ 0%nat := (live_roles Mdl s1) ]}, _. *)
+  (*   iSplitL "Hfuela"; first by rewrite /auth_fuel_is /= fmap_gset_to_gmap //. *)
+  (*   iSplitL "Hmapa"; first by rewrite /auth_mapping_is /= map_fmap_singleton //. *)
+  (*   iSplit; first done. *)
+  (*   iSplit; iPureIntro; [|split]. *)
+  (*   - intros ρ tid. rewrite lookup_gset_to_gmap_Some. *)
+  (*     setoid_rewrite lookup_singleton_Some. split; naive_solver. *)
+  (*   - intros tid Hlocs. rewrite lookup_singleton_ne //. compute in Hlocs. set_solver. *)
+  (*   - rewrite dom_gset_to_gmap. set_solver. } *)
+  iSpecialize ("Hwp" with "Hσ Hmodf Hfr [Hfuelf Hmapf]").
+  { rewrite /has_fuels /frag_mapping_is /= map_fmap_singleton. iFrame.
+    iAssert ([∗ set] ρ ∈ live_roles M s1, ρ ↦F (LM.(lm_fl) s1))%I with "[Hfuelf]" as "H".
+    - unfold frag_fuel_is. setoid_rewrite map_fmap_singleton.
+      rewrite -big_opS_own //. iApply (own_proper with "Hfuelf").
+      rewrite -big_opS_auth_frag. f_equiv. rewrite gset_to_gmap_singletons //.
+    - rewrite dom_gset_to_gmap. iFrame.
+      iApply (big_sepS_mono with "H"). iIntros (ρ Hin) "H".
+      iExists _. iFrame. iPureIntro. apply lookup_gset_to_gmap_Some. done. }
+  iDestruct "Hwp" as ">[Hwp H]".
+  iModIntro. iFrame "Hwp".
+  iSplitL "Hgen Hmoda Hmapa Hfuela HFR".
+  { unfold state_interp. simpl. iFrame. iExists {[ 0%nat := (live_roles M s1) ]}, _.
+    iSplitL "Hfuela"; first by rewrite /auth_fuel_is /= fmap_gset_to_gmap //.
+    iSplitL "Hmapa"; first by rewrite /auth_mapping_is /= map_fmap_singleton //.
+    iSplit; first done.
+    iSplit; iPureIntro; [|split].
+    - intros ρ tid. rewrite lookup_gset_to_gmap_Some.
+      setoid_rewrite lookup_singleton_Some. split; naive_solver.
+    - intros tid Hlocs. rewrite lookup_singleton_ne //. compute in Hlocs. set_solver.
+    - rewrite dom_gset_to_gmap. set_solver. }
+  iIntros (ex atr c Hvalex Hstartex Hstartatr Hendex Hcontr Hstuck Hequiv) "Hsi Hposts".
+  assert ( ∀ (ex' : finite_trace (cfg heap_lang) (olocale heap_lang)) (atr' : auxiliary_trace LM) (oζ : olocale heap_lang) (ℓ : mlabel LM),
+   trace_contract ex oζ ex' → trace_contract atr ℓ atr' → ξ ex' (map_underlying_trace atr')) as Hcontr'.
+  { intros ex' atr' oζ ℓ H1 H2. cut (sim_rel_with_user LM ξ ex' atr'); eauto. rewrite /sim_rel_with_user. intros [??]. done. }
+  iSpecialize ("H" $! ex atr c Hvalex Hstartex Hstartatr Hendex Hcontr' Hstuck).
+  unfold sim_rel_with_user.
+  iAssert (|={⊤}=> ⌜ξ ex (map_underlying_trace atr)⌝ ∗ state_interp ex atr ∗ posts_of c.1
+               ((λ _ : language.val heap_lang, 0 ↦M ∅)
+                :: ((λ '(tnew, e), fork_post (language.locale_of tnew e)) <$>
+                    prefixes_from [e1] (drop (length [e1]) c.1))))%I with "[Hsi H Hposts]" as "H".
+  { iApply fupd_plain_keep_l. iFrame. iIntros "[Hsi Hposts]".
+    iSpecialize ("H" with "Hsi Hposts").
+    by iApply fupd_plain_mask_empty. }
+  iMod "H" as "[H1 [Hsi Hposts]]".
+  destruct ex as [c'|ex' tid (e, σ)].
+  - (* We need to prove that the initial state satisfies the property *)
+    destruct atr as [δ|???]; last by inversion Hvalex. simpl.
+    have Heq1 := trace_singleton_ends_in_inv _ _ Hendex.
+    have Heq3 := trace_singleton_starts_in_inv _ _ Hstartex.
+    have Heq4 := trace_singleton_starts_in_inv _ _ Hstartex.
+    pose proof (trace_singleton_starts_in_inv _ _ Hstartatr). simpl.
+    simplify_eq.
+    iApply (fupd_mask_weaken ∅); first set_solver. iIntros "_ !>".
+    assert (∀ (ρ : fmrole M) (tid : nat),
+               ls_mapping (initial_ls (LM := LM) s1 0%nat) !! ρ = Some tid →
+               is_Some (([e1], σ1).1 !! tid)) as HA.
+    { simpl. intros ρ tid Hsome. apply lookup_gset_to_gmap_Some in Hsome as [??].
+      simplify_eq. by eexists _. }
+    iSplit; last done. iClear "H1".
+    iSplit; first done.
+    destruct (to_val e1) as [v1|] eqn:Heq.
+    + iSplit.
+      { iPureIntro. intros ρ tid Hinit.
+        simpl in *. apply lookup_gset_to_gmap_Some in Hinit as [_ <-].
+        rewrite /from_locale //. }
+      iIntros (tid e Hsome Hnoval ρ). destruct tid; last done.
+      simpl in Hsome. compute in Hsome. simplify_eq. simpl.
+      iAssert (0%nat ↦M ∅) with "[Hposts]" as "Hem".
+      { rewrite /= Heq /fmap /=. by iDestruct "Hposts" as "[??]". }
+      iDestruct "Hsi" as "(_&_&Hsi)".
+      iDestruct "Hsi" as "(%m&%FR'&Hfuela&Hmapa&HFR&%Hinvmap&%Hsmall&Hmodel&HfrFR)".
+      iDestruct (frag_mapping_same 0%nat m with "[Hmapa] Hem") as "%H"; first done.
+      iPureIntro. by eapply no_locale_empty.
+    + iSplit; iPureIntro.
+      { simpl. intros ρ tid Hsome. apply lookup_gset_to_gmap_Some in Hsome as [??].
+        simplify_eq. by eexists _. }
+      intros tid e Hsome Hval' ρ.
+      destruct tid as [|tid]; rewrite /from_locale /= in Hsome; by simplify_eq.
+  - (* We need to prove that that the property is preserved *)
+    destruct atr as [|atr' ℓ δ]; first by inversion Hvalex.
+    (* rewrite (trace_singleton_ends_in_inv _ _ Hendex); last exact unit. *)
+    specialize (Hcontr ex' atr' tid ℓ).
+    have H: trace_contract (trace_extend ex' tid (e, σ)) tid ex' by eexists.
+    have H': trace_contract (trace_extend atr' ℓ δ) ℓ atr' by eexists.
+    specialize (Hcontr H H') as Hvs. clear H H' Hcontr.
+    (* destruct Hvalex as (Hlm & Hlt & Hts). *)
+    have H: trace_ends_in ex' (trace_last ex') by eexists.
+    have H': trace_ends_in atr' (trace_last atr') by eexists.
+    iApply (fupd_mask_weaken ∅); first set_solver. iIntros "_ !>".
+    apply (trace_singleton_ends_in_inv (L := unit)) in Hendex.
+    simpl in *. simplify_eq.
+    iDestruct "Hsi" as "((%&%&%Htids)&_&Hsi)".
+    iDestruct "Hsi" as "(%m&%&Hfuela&Hmapa&?&%Hinvmap&%Hsmall&Hmodel&?)".
+    iSplit; [|done].
+    iSplit; [done|].
+    iSplit.
+    + iPureIntro. intros ρ tid' Hsome. simpl. unfold tids_smaller in Htids. eapply Htids. done.
+    + iIntros (tid' e' Hsome Hnoval ρ). simpl.
+      iAssert (tid' ↦M ∅) with "[Hposts]" as "H".
+      { destruct (to_val e') as [?|] eqn:Heq; last done.
+        iApply posts_of_empty_mapping => //.
+        apply from_locale_lookup =>//. }
+      iDestruct (frag_mapping_same tid' m with "Hmapa H") as "%Hlk".
+      { rewrite /auth_mapping_is. iPureIntro. by eapply no_locale_empty. }
+Qed.
 
 
 (* The model is finitely branching *)
@@ -63,42 +308,6 @@ Proof.
     rewrite /role_enabled_model in Hfair. destruct t; destruct ρ; set_solver.
   - by exists m.
 Qed.
-
-(* Lemma yesno_mdl_scheduled ρ (mtr : yesno_mtrace) : *)
-(*   (* (∀ ρ, fair_model_trace ρ mtr) → *) *)
-(*   ∀ n, ∃ m, pred_at mtr (n+m) (λ _ ℓ, ℓ = Some (Some ρ)). *)
-(* Proof. *)
-
-
-From Paco Require Import paco1 paco2 pacotac.
-
-(* TODO: move to fairness.v *)
-Lemma mtrace_valid_after `{M : FairModel} (mtr mtr' : mtrace M) k :
-  after k mtr = Some mtr' → mtrace_valid mtr → mtrace_valid mtr'.
-Proof.
-  revert mtr mtr'.
-  induction k; intros mtr mtr' Hafter Hvalid.
-  { destruct mtr'; simpl in *; by simplify_eq. }
-  punfold Hvalid.
-  inversion Hvalid as [|??? Htrans Hval']; simplify_eq.
-  eapply IHk; [done|].
-  by inversion Hval'.
-Qed.
-
-Lemma even_odd_False n : Nat.even n → Nat.odd n → False.
-Proof.
-  intros Heven Hodd. rewrite -Nat.negb_odd in Heven.
-  apply Is_true_true_1 in Heven.
-  apply Is_true_true_1 in Hodd.
-  rewrite Hodd in Heven.
-  done.
-Qed.
-
-Lemma even_not_odd n : Nat.even n → ¬ Nat.odd n.
-Proof. intros Heven Hodd. by eapply even_odd_False. Qed.
-
-Lemma odd_not_even n : Nat.odd n → ¬ Nat.even n.
-Proof. intros Heven Hodd. by eapply even_odd_False. Qed.
 
 Lemma yesno_mdl_noprogress_Y n m (mtr : yesno_mtrace) :
   infinite_trace mtr →
@@ -236,13 +445,6 @@ Proof.
   - by apply odd_not_even in Hodd.
 Qed.
 
-Lemma infinite_trace_after'' {S T} n (tr tr' : trace S T) :
-  after n tr = Some tr' → infinite_trace tr → infinite_trace tr'.
-Proof.
-  intros Hafter Hinf m. specialize (Hinf (n+m)).
-  rewrite after_sum' in Hinf. rewrite Hafter in Hinf. done.
-Qed.
-
 Theorem yesno_mdl_progresses (mtr : yesno_mtrace) :
   infinite_trace mtr →
   mtrace_valid mtr →
@@ -278,45 +480,7 @@ Proof.
     rewrite pred_at_sum. rewrite Hafter. done.
 Qed.
 
-Lemma trace_eventually_cons {S T} s l (tr : trace S T) P :
-  trace_eventually tr P → trace_eventually (s -[l]-> tr) P.
-Proof. intros [n HP]. by exists (Datatypes.S n). Qed.
-
-(* Definition yesno_aux_progress n b (auxtr : auxtrace the_model) := *)
-(*   trace_eventually auxtr (ls_under ∘ (λ s _, s = (n,b))). *)
-Lemma trace_eventually_stutter_preserves `(LM : LiveModel Λ FM)
-      (mtr : mtrace FM)
-      (auxtr : auxtrace LM) P :
-  upto_stutter ls_under Ul auxtr mtr →
-  trace_eventually mtr P →
-  trace_eventually auxtr (λ s l, P (ls_under s) (l ≫= Ul)).
-Proof.
-  intros Hstutter [n Heventually].
-  revert mtr auxtr Hstutter Heventually.
-  induction n as [|n IHn]; intros mtr auxtr Hstutter Heventually.
-  - punfold Hstutter; [|apply upto_stutter_mono].
-    induction Hstutter.
-    + rewrite /pred_at in Heventually. simpl in *. exists 0. rewrite /pred_at. simpl in *. done.
-    + destruct (IHHstutter Heventually) as [n Heventually'].
-      exists (1 + n). rewrite /pred_at. rewrite after_sum'. simpl.
-      done.
-    + rewrite /pred_at in Heventually. simpl in *. exists 0. rewrite /pred_at. simpl.
-      simplify_eq. rewrite H0. done.
-  - punfold Hstutter; [|apply upto_stutter_mono].
-    induction Hstutter.
-    + rewrite /pred_at in Heventually. simpl in *. exists 0. rewrite /pred_at. simpl in *. done.
-    + destruct (IHHstutter Heventually) as [n' Heventually'].
-      exists (1 + n'). rewrite /pred_at. rewrite after_sum'. simpl.
-      done.
-    + apply trace_eventually_cons.
-      assert (pred_at str n P) as Heventually'.
-      { rewrite /pred_at in Heventually.
-        simpl in *. done. }
-      eapply IHn; [|done].
-      rewrite /upaco2 in H1. destruct H1; [done|done].
-Qed.
-
-(* TODO: better definition *)
+(* TODO: Better definition *)
 Definition yesno_aux_progress (auxtr : auxtrace the_model) :=
   ∀ n, ∃ m, pred_at auxtr m (λ s l, (λ s' _, s' = n) (ls_under s) (l ≫= Ul)).
 
@@ -326,98 +490,35 @@ Lemma yesno_mtr_aux_progress_preserved
   upto_stutter ls_under Ul auxtr mtr →
   yesno_mdl_progress mtr → yesno_aux_progress auxtr.
 Proof.
-  intros Hstutter Hmtr.
-  intros n. apply (trace_eventually_stutter_preserves _ mtr auxtr (λ s' _, s' = n)).
-  - done.
-  - apply Hmtr.
+  intros Hstutter Hmtr n. specialize (Hmtr n).
+  by apply (trace_eventually_stutter_preserves _ mtr auxtr (λ s' _, s' = n)).
 Qed.
 
-(* Defining this requires exposing the location in the state *)
-(* Definition yesno_ex_progress (tr : heap_lang_extrace) := *)
-(*   ∀ n b, ∃ m, pred_at tr m (λ s _, s.2 !! ??? = Some ???). *)
 Definition yesno_ex_progress (l:loc) (tr : heap_lang_extrace) :=
   ∀ (n:nat), ∃ m, pred_at tr m (λ s _, heap s.2 !! l = Some #n).
 
-Definition ξ_yesno' (l : loc) (extr : execution_trace heap_lang)
+Definition ξ_yesno_model_match (l : loc) (c : cfg heap_lang) (δ : the_fair_model) :=
+  ∃ (N:nat), heap c.2 !! l = Some #N ∧ δ = N.
+
+Definition ξ_yesno_steps (l : loc) (c : cfg heap_lang) (δ : the_fair_model) :=
+  Forall (λ e, is_Some $ to_val e) c.1 → False.
+
+Definition ξ_yesno (l : loc) (c : cfg heap_lang) (δ : the_fair_model) :=
+  ξ_yesno_steps l c δ ∧
+  ξ_yesno_model_match l c δ.
+
+Definition ξ_yesno_trace (l : loc) (extr : execution_trace heap_lang)
            (auxtr : finite_trace the_fair_model (option YN)) :=
-  ∃ (N:nat), heap (trace_last extr).2 !! l = Some #N ∧ (trace_last auxtr) = N.
+  ξ_yesno l (trace_last extr) (trace_last auxtr).
 
-Definition ξ_yesno (l : loc) (extr : heap_lang_extrace) (auxtr : auxtrace the_model) :=
-  ∀ n, ∃ (N:nat),
-    pred_at extr n (λ σ _, heap σ.2 !! l = Some #N) ∧
-    pred_at auxtr n (λ δ _, ls_under δ = N).
-
-Lemma yesno_aux_ex_progress_preserved l (extr : heap_lang_extrace) (auxtr : auxtrace the_model) :
-  ξ_yesno l extr auxtr → yesno_aux_progress auxtr → yesno_ex_progress l extr.
-Proof.
-  intros Hξ Hauxtr.
-  intros n.
-  specialize (Hauxtr n).
-  destruct Hauxtr as [m Hauxtr].
-  exists m.
-  destruct (Hξ m) as [N [Hextr' Hauxtr']].
-  rewrite /pred_at.
-  rewrite /pred_at in Hauxtr.
-  rewrite /pred_at in Hauxtr'.
-  rewrite /pred_at in Hextr'.
-  destruct (after m auxtr); [|done].
-  destruct (after m extr); [|done].
-  destruct t; destruct t0; by simplify_eq.
-Qed.
-
-(* TODO: move *)
-Lemma traces_match_infinite_trace {L1 L2 S1 S2: Type}
-      (Rℓ: L1 -> L2 -> Prop) (Rs: S1 -> S2 -> Prop)
-      (trans1: S1 -> L1 -> S1 -> Prop)
-      (trans2: S2 -> L2 -> S2 -> Prop) tr1 tr2 :
-  traces_match Rℓ Rs trans1 trans2 tr1 tr2 → infinite_trace tr1 → infinite_trace tr2.
-Proof.
-  intros Hmatch Hinf n.
-  specialize (Hinf n) as [tr' Hafter].
-  apply traces_match_flip in Hmatch.
-  by eapply traces_match_after in Hafter as [tr'' [Hafter' _]].
-Qed.
-
-Lemma upto_stutter_infinite_trace {St S' L L': Type} (Us: St -> S') (Ul: L -> option L')
- tr1 tr2 :
-  upto_stutter Us Ul tr1 tr2 → infinite_trace tr1 → infinite_trace tr2.
-Proof.
-  intros Hstutter Hinf n.
-  revert tr1 tr2 Hstutter Hinf.
-  induction n as [|n IHn]; intros tr1 tr2 Hstutter Hinf.
-  - punfold Hstutter. apply upto_stutter_mono.
-  - punfold Hstutter; [|apply upto_stutter_mono].
-    induction Hstutter.
-    + specialize (Hinf (1 + n)).
-      rewrite after_sum' in Hinf. simpl in *. apply is_Some_None in Hinf. done.
-    + apply IHHstutter.
-      intros m. specialize (Hinf (1 + m)).
-      rewrite after_sum' in Hinf. simpl in *. done.
-    + simpl. eapply (IHn btr str); [by destruct H1|].
-      intros m. specialize (Hinf (1 + m)).
-      rewrite after_sum' in Hinf. simpl in *. done.
-Qed.
-
-Lemma rel_finitary_sim_rel_with_user_sim_rel `{LM:LiveModel Λ Mdl}
-      `{EqDecision (mstate LM)} `{EqDecision (mlabel LM)}
-      `{Countable (locale Λ)} ξ :
-  rel_finitary (sim_rel LM) → rel_finitary (sim_rel_with_user LM ξ).
-Proof.
-  intros Hrel. eapply rel_finitary_impl; [|done]. by intros ex aux [Hsim _].
-Qed.
-
-(* TODO *)
 Instance the_model_mstate_countable : EqDecision (mstate the_model).
-Proof. Admitted.
-
+Proof. intros x y. apply make_decision. Qed.
 Instance the_model_mlabel_countable : EqDecision (mlabel the_model).
-Proof. Admitted.
+Proof. solve_decision. Qed.
 
-(** Derive that program is related to model by
-    [sim_rel_with_user cn_model (ξ_cn l) using Trillium adequacy *)
 Lemma yesno_incr_sim l :
   continued_simulation
-    (sim_rel_with_user the_model (ξ_yesno' l))
+    (sim_rel_with_user the_model (ξ_yesno_trace l))
     (trace_singleton ([start #l],
                         {| heap := {[l:=#0]};
                            used_proph_id := ∅ |}))
@@ -462,21 +563,125 @@ Proof.
       rewrite left_id. done. }
     iApply (start_spec with "[$Hf $Hyes_at $Hno_at $Hinv]"); [lia|].
     by iIntros "!>?". }
-  iIntros (extr auxtr c) "??????[?[Hσ Hδ]]".
-  iInv "Hinv" as (M) "(>HFR & >Hmod & >Hn & Hauths)" "Hclose".
+  iIntros (extr auxtr c) "_ _ _ %Hends _ _ [_ [Hσ Hδ]]Hposts".
+  iInv "Hinv" as (M) "(_ & >Hmod & >Hn & _)" "Hclose".
   iApply fupd_mask_intro; [set_solver|].
   iIntros "Hclose'".
   iDestruct (gen_heap_valid with "Hσ Hn") as %Hn.
-  iDestruct "Hδ" as (??) "(?&?&?&?&?&Hδ&?)".
+  iDestruct "Hδ" as (??) "(_&_&_&_&_&Hδ&_)".
   iDestruct (model_agree with "Hδ Hmod") as %Hn'.
-  iPureIntro. exists M. split; [done|].
-  rewrite -Hn'. by destruct auxtr.
+  iSplitL; last first.
+  { iPureIntro.
+    exists M. split; [done|].
+    rewrite -Hn'. by destruct auxtr. }
+  rewrite /trace_ends_in in Hends.
+  rewrite Hends.
+  rewrite bi.pure_impl.
+  iIntros "%Hall".
+  rewrite !big_sepL_omap.
+  rewrite !big_sepL_zip_with.
+  simpl.
+Admitted.
+
+Lemma yesno_aux_ex_progress_preserved l (extr : heap_lang_extrace) (auxtr : auxtrace the_model) :
+  traces_match labels_match
+               (λ (x0 : cfg heap_lang) (x1 : lm_ls the_model),
+                  live_tids x0 x1 ∧ ξ_yesno l x0 x1) locale_step
+  (lm_ls_trans the_model) extr auxtr →
+  yesno_aux_progress auxtr → yesno_ex_progress l extr.
+Proof.
+  intros Hξ Hauxtr.
+  intros n.
+  specialize (Hauxtr n).
+  rewrite /pred_at in Hauxtr.
+  destruct Hauxtr as [m Hauxtr].
+  destruct (after m auxtr) eqn:Heqn; [|done].
+  eapply traces_match_after in Hξ as [extr' [Hafter' Hextr']]; [|done].
+  exists m. rewrite /pred_at. rewrite Hafter'.
+  inversion Hextr'; simplify_eq.
+  - destruct H as [? [? [n [? ?]]]]. simplify_eq. done.
+  - destruct H0 as [? [? [n [? ?]]]]. simplify_eq. done.
 Qed.
 
 Theorem yesno_ex_progresses (l:loc) (extr : heap_lang_extrace) :
   extrace_valid extr →
   (∀ tid, fair_ex tid extr) →
-  (trfirst extr).1 = [start #l] →
+  trfirst extr = ([start #l],
+                        {| heap := {[l:=#0]};
+                           used_proph_id := ∅ |}) →
   yesno_ex_progress l extr.
 Proof.
+  intros Hvalid Hfair Hfirst.
+  pose proof (yesno_incr_sim l) as Hsim.
+
+  assert (∃ iatr,
+             valid_inf_system_trace
+               (continued_simulation (sim_rel_with_user the_model (ξ_yesno_trace l)))
+               (trace_singleton (trfirst extr))
+               (trace_singleton (initial_ls (LM:=the_model) 0 0))
+               (from_trace extr)
+               iatr) as [iatr Hiatr].
+  { eexists _. eapply produced_inf_aux_trace_valid_inf. econstructor.
+    Unshelve.
+    - rewrite Hfirst. done.
+    - eapply from_trace_preserves_validity; eauto; first econstructor. }
+
+  assert (∃ (auxtr : auxtrace the_model),
+             traces_match labels_match
+               (live_tids /2\ (ξ_yesno l))
+               locale_step
+               the_model.(lm_ls_trans) extr auxtr) as [auxtr Hmatch_strong].
+  { exists (to_trace (initial_ls (LM := the_model) 0 0 ) iatr).
+    eapply (valid_inf_system_trace_implies_traces_match_strong
+              (continued_simulation (sim_rel_with_user the_model (ξ_yesno_trace l)))); eauto.
+    - intros ? ? ?%continued_simulation_rel. by destruct H as [[_ H] _].
+    - intros ? ? ?%continued_simulation_rel. by destruct H as [[H _] _].
+    - intros extr' auxtr' ?%continued_simulation_rel.
+      destruct H as [_ [H1 H2]].
+      split; [done|].
+      destruct H2 as [n [H21 H22]].
+      exists n. split; [done|]. by destruct auxtr'.
+    - by apply from_trace_spec.
+    - by apply to_trace_spec. }
+
+  assert (exaux_traces_match extr auxtr) as Hmatch.
+  { eapply traces_match_impl; [| |done].
+    - done.
+    - by intros ?? [? ?]. }
+  have Hstutter:=Hmatch.
+  apply can_destutter_auxtr in Hstutter; last first.
+  { intros ?? Hstep. inversion Hstep. done. }
+  destruct Hstutter as [mtr Hupto].
+
+  assert (infinite_trace extr) as Hinf by admit.
+
+  have Hfairaux := fairness_preserved extr auxtr Hinf Hmatch Hfair.
+  have Hvalaux := exaux_preserves_validity extr auxtr Hmatch.
+  have Hfairm := upto_stutter_fairness auxtr mtr Hupto Hfairaux.
+  have Hmtrvalid := upto_preserves_validity auxtr mtr Hupto Hvalaux.
+
+  pose proof (fairness_preserved extr auxtr Hinf Hmatch Hfair) as Hfair'.
+  pose proof (upto_stutter_fairness auxtr mtr Hupto Hfair') as Hfair''.
+
+  assert (infinite_trace mtr) as Hinf''.
+  { eapply upto_stutter_infinite_trace; [done|].
+    by eapply traces_match_infinite_trace. }
+  assert (mtrace_valid mtr) as Hvalid''.
+  { eapply upto_preserves_validity; [done|].
+    by eapply exaux_preserves_validity. }
+
+  (* TODO: Improve proof *)
+  assert (trfirst mtr = 0) as Hfirst''.
+  { apply traces_match_first in Hmatch_strong.
+    destruct Hmatch_strong as [_ [_ [n [Hσ Hmdl]]]].
+    rewrite Hfirst in Hσ. simpl in *. rewrite lookup_insert in Hσ.
+    simplify_eq. punfold Hupto; [|by apply upto_stutter_mono'].
+    assert (0 = ls_under (trfirst auxtr)) as Hσ' by lia.
+    inversion Hupto; simplify_eq;
+    by rewrite Hσ'. }
+
+  pose proof (yesno_mdl_progresses mtr Hinf'' Hvalid'' Hfair'' Hfirst'')
+    as Hprogress.
+  eapply (yesno_aux_ex_progress_preserved l _ auxtr); [done|].
+  by eapply yesno_mtr_aux_progress_preserved.
 Admitted.
